disk-betree/Graph.dfy
@@ -6,4 +6,9 @@ abstract module Graph {
   function Successors(node: Node) : iset<Reference>
 
   type Graph = imap<Reference, Node>
+
+  // TODO Transactable is a more natural place for this
+  datatype Op =
+    | AllocOp(ref: Reference, block: Node)
+    | WriteOp(ref: Reference, block: Node)
 }
