disk-betree/Transactable.dfy
@@ -1,0 +1,109 @@
+include "../lib/sequences.dfy"
+include "Graph.dfy"
+
+abstract module Transactable {
+  import opened Sequences
+
+  import G : Graph
+
+  type Reference = G.Reference
+  type Node = G.Node
+  type Op = G.Op
+
+  type Constants(!new)
+  type Variables(!new)
+
+  predicate OpStep(k: Constants, s: Variables, s': Variables, op: Op)
+
+  predicate IsStatePath(k: Constants, s: Variables, s': Variables, ops: seq<Op>, path: seq<Variables>)
+  {
+    && |path| == |ops| + 1
+    && path[0] == s
+    && Last(path) == s'
+    && (forall i :: 0 <= i < |ops| ==> OpStep(k, path[i], path[i+1], ops[i]))
+  }
+
+  lemma Transaction1Steps(k: Constants, s: Variables, s': Variables, ops: seq<Op>)
+  ensures (
+    && 0 < |ops|
+    && (exists path: seq<Variables> :: IsStatePath(k, s, s', ops, path))
+    && |ops| == 1
+  ) ==>
+      && OpStep(k, s, s', ops[0])
+  {
+    if (
+        && 0 < |ops|
+        && (exists path: seq<Variables> :: IsStatePath(k, s, s', ops, path))
+        && |ops| == 1)
+    {
+      var path :| IsStatePath(k, s, s', ops, path);
+      assert OpStep(k, s, s', ops[0]);
+    }
+  }
+
+
+  lemma Transaction2Steps(k: Constants, s: Variables, s': Variables, ops: seq<Op>)
+  ensures (
+    && 0 < |ops|
+    && (exists path: seq<Variables> :: IsStatePath(k, s, s', ops, path))
+    && |ops| == 2
+  ) ==>
+      exists sint ::
+      && OpStep(k, s, sint, ops[0])
+      && OpStep(k, sint, s', ops[1])
+  {
+    if (
+        && 0 < |ops|
+        && (exists path: seq<Variables> :: IsStatePath(k, s, s', ops, path))
+        &&| ops| == 2)
+    {
+      var path :| IsStatePath(k, s, s', ops, path);
+      var sint := path[1];
+      assert OpStep(k, s, sint, ops[0]);
+      assert OpStep(k, sint, s', ops[1]);
+    }
+  }
+
+  lemma Transaction3Steps(k: Constants, s: Variables, s': Variables, ops: seq<Op>)
+  ensures (
+    && 0 < |ops|
+    && (exists path: seq<Variables> :: IsStatePath(k, s, s', ops, path))
+    && |ops| == 3
+  ) ==>
+      exists sint, sint' ::
+      && OpStep(k, s, sint, ops[0])
+      && OpStep(k, sint, sint', ops[1])
+      && OpStep(k, sint', s', ops[2])
+  {
+    if (
+        && 0 < |ops|
+        && (exists path: seq<Variables> :: IsStatePath(k, s, s', ops, path))
+        && |ops| == 3)
+    {
+      var path :| IsStatePath(k, s, s', ops, path);
+      var sint := path[1];
+      var sint' := path[2];
+      assert OpStep(k, s, sint, ops[0]);
+      assert OpStep(k, sint, sint', ops[1]);
+      assert OpStep(k, sint', s', ops[2]);
+    }
+  }
+  
+  predicate Transaction(k: Constants, s: Variables, s': Variables, ops: seq<Op>)
+    ensures Transaction(k, s, s', ops) && |ops| == 1 ==>
+      && OpStep(k, s, s', ops[0])
+    ensures Transaction(k, s, s', ops) && |ops| == 2 ==> exists sint ::
+      && OpStep(k, s, sint, ops[0])
+      && OpStep(k, sint, s', ops[1])
+    ensures Transaction(k, s, s', ops) && |ops| == 3 ==> exists sint, sint' ::
+      && OpStep(k, s, sint, ops[0])
+      && OpStep(k, sint, sint', ops[1])
+      && OpStep(k, sint', s', ops[2])
+  {
+    Transaction1Steps(k, s, s', ops);
+    Transaction2Steps(k, s, s', ops);
+    Transaction3Steps(k, s, s', ops);
+    && 0 < |ops|
+    && (exists path: seq<Variables> :: IsStatePath(k, s, s', ops, path))
+  }
+}
